Progress pushing results up to gcm_encrypt_LE. Still need to handle the extra bytes cases

vale/code/crypto/aes/GCM.fst
@@ -13,6 +13,7 @@ open FStar.Mul
 open FStar.Seq
 open Words_s
 open Words.Seq_s
+open FStar.Calc
 
 let gcm_encrypt_LE_fst_helper (iv_enc iv_BE:quad32) (plain auth cipher:seq nat8) (alg:algorithm) (key:seq nat32) : Lemma
   (requires
@@ -65,6 +66,296 @@ let gcm_encrypt_LE_snd_helper (iv_BE length_quad32 hash mac:quad32) (plain auth 
   //be_bytes_to_quad32_to_bytes iv_BE;
   //let t = snd (gcm_encrypt_LE alg (seq_nat32_to_seq_nat8_LE key) (be_quad32_to_bytes iv_BE) plain auth) in
   //()
+
+
+
+#reset-options "--z3rlimit 10"
+let gcm_blocks_helper_enc (alg:algorithm) (key:seq nat32)
+                   (p128x6 p128 p_bytes c128x6 c128 c_bytes:seq quad32)
+                   (auth_bytes:seq nat8)
+                   (p_num_bytes:nat)
+                   (iv_BE:quad32) : Lemma
+  (requires // Required by gcm_blocks
+           0 < p_num_bytes /\
+           4096 * (length p128x6 + length p128 + 1) * 16 < pow2_32 /\
+           length p128x6 * 16 + length p128 * 16 <= p_num_bytes /\
+           p_num_bytes < length p128x6 * 16 + length p128 * 16 + 16 /\
+           length p128x6 == length c128x6 /\
+           length p128 == length c128 /\
+           length p_bytes == 1 /\
+           length c_bytes == 1 /\
+           4096 * (length auth_bytes) < pow2_32 /\
+           is_aes_key_LE alg key /\
+
+           // Ensured by gcm_blocks
+           8 * p_num_bytes < pow2_32 /\ 
+          (let ctr_BE_2:quad32 = Mkfour 2 iv_BE.lo1 iv_BE.hi2 iv_BE.hi3 in
+           let plain:seq quad32 = 
+             if p_num_bytes > (length p128x6 + length p128) * 16 then
+               append (append p128x6 p128) p_bytes
+             else
+               append p128x6 p128
+           in
+           let cipher:seq quad32 =
+             if p_num_bytes > (length p128x6 + length p128) * 16 then
+               append (append c128x6 c128) c_bytes
+             else
+               append c128x6 c128
+           in
+           let cipher_bound:nat = length p128x6 + length p128 +
+             (if p_num_bytes > (length p128x6 + length p128) * 16 then 1 else 0)
+           in
+           gctr_partial_opaque alg cipher_bound plain cipher key ctr_BE_2
+           ))
+  (ensures (let plain:seq quad32 = 
+             if p_num_bytes > (length p128x6 + length p128) * 16 then
+               append (append p128x6 p128) p_bytes
+             else
+               append p128x6 p128
+           in
+           let cipher:seq quad32 =
+             if p_num_bytes > (length p128x6 + length p128) * 16 then
+               append (append c128x6 c128) c_bytes
+             else
+               append c128x6 c128
+           in
+           let ctr_BE_2:quad32 = Mkfour 2 iv_BE.lo1 iv_BE.hi2 iv_BE.hi3 in
+           let plain_bytes = slice (le_seq_quad32_to_bytes plain) 0 p_num_bytes in
+           let cipher_bytes = slice (le_seq_quad32_to_bytes cipher) 0 p_num_bytes in
+           //cipher_bytes == gctr_encrypt_LE ctr_BE_2 plain_bytes alg key))
+           cipher_bytes == fst (gcm_encrypt_LE alg (seq_nat32_to_seq_nat8_LE key) (be_quad32_to_bytes iv_BE) plain_bytes auth_bytes)))
+  =
+  let ctr_BE_2:quad32 = Mkfour 2 iv_BE.lo1 iv_BE.hi2 iv_BE.hi3 in
+  let plain:seq quad32 = 
+    if p_num_bytes > (length p128x6 + length p128) * 16 then
+       append (append p128x6 p128) p_bytes
+    else
+      append p128x6 p128
+  in
+  let cipher:seq quad32 =
+    if p_num_bytes > (length p128x6 + length p128) * 16 then
+       append (append c128x6 c128) c_bytes
+    else
+      append c128x6 c128
+  in
+  let cipher_bound:nat = length p128x6 + length p128 +
+    (if p_num_bytes > (length p128x6 + length p128) * 16 then 1 else 0)
+  in
+  let plain_bytes = slice (le_seq_quad32_to_bytes plain) 0 p_num_bytes in
+  let cipher_bytes = slice (le_seq_quad32_to_bytes cipher) 0 p_num_bytes in
+  gctr_partial_opaque_completed alg plain cipher key ctr_BE_2;
+  if p_num_bytes > (length p128x6 + length p128) * 16 then (
+    reveal_opaque gctr_partial;
+    assert (gctr_partial_opaque alg (length p128x6 + length p128) plain cipher key ctr_BE_2);
+    assert (equal (slice plain 0 (length p128x6 + length p128))
+                  (slice (append p128x6 p128) 0 (length p128x6 + length p128)));
+    assert (equal (slice cipher 0 (length p128x6 + length p128))
+                  (slice (append c128x6 c128) 0 (length p128x6 + length p128)));                  
+    gctr_partial_opaque_ignores_postfix
+      alg (length p128x6 + length p128)
+      plain (append p128x6 p128)
+      cipher (append c128x6 c128) 
+      key ctr_BE_2;
+    assert (gctr_partial_opaque alg (length p128x6 + length p128) (append p128x6 p128) (append c128x6 c128) key ctr_BE_2);
+    gctr_partial_opaque_completed alg (append p128x6 p128) (append c128x6 c128) key ctr_BE_2; 
+    let num_blocks = p_num_bytes / 16 in
+    assert(index cipher num_blocks == quad32_xor (index plain num_blocks) (aes_encrypt_BE alg key (inc32 ctr_BE_2 num_blocks)));
+    gctr_encrypt_block_offset ctr_BE_2 (index plain num_blocks) alg key num_blocks;
+    assert( gctr_encrypt_block ctr_BE_2 (index plain num_blocks) alg key num_blocks ==
+            gctr_encrypt_block (inc32 ctr_BE_2 num_blocks) (index plain num_blocks) alg key 0);
+    reveal_opaque aes_encrypt_LE_def;
+    gctr_partial_to_full_advanced ctr_BE_2 plain cipher alg key p_num_bytes;
+    assert (cipher_bytes == gctr_encrypt_LE ctr_BE_2 plain_bytes alg key)
+  ) else (
+    gctr_partial_to_full_basic ctr_BE_2 plain alg key cipher;
+    assert (le_seq_quad32_to_bytes cipher == gctr_encrypt_LE ctr_BE_2 (le_seq_quad32_to_bytes plain) alg key);
+    let plain_bytes = slice (le_seq_quad32_to_bytes plain) 0 p_num_bytes in
+    let cipher_bytes = slice (le_seq_quad32_to_bytes cipher) 0 p_num_bytes in
+    assert (equal plain_bytes (le_seq_quad32_to_bytes plain));
+    assert (equal cipher_bytes (le_seq_quad32_to_bytes cipher));
+    assert (cipher_bytes == gctr_encrypt_LE ctr_BE_2 plain_bytes alg key)
+  );
+  gcm_encrypt_LE_fst_helper ctr_BE_2 iv_BE plain_bytes auth_bytes cipher_bytes alg key;
+  ()
+
+let gcm_blocks_helper (alg:algorithm) (key:seq nat32)
+                   (a128 a_bytes p128x6 p128 p_bytes c128x6 c128 c_bytes:seq quad32)
+                   (p_num_bytes a_num_bytes:nat)
+                   (iv_BE h enc_hash length_quad:quad32) : Lemma
+  (requires // Required by gcm_blocks
+           0 < p_num_bytes /\
+           4096 * (length p128x6 + length p128 + 1) * 16 < pow2_32 /\
+           length p128x6 * 16 + length p128 * 16 <= p_num_bytes /\
+           p_num_bytes < length p128x6 * 16 + length p128 * 16 + 16 /\
+           length a128 * 16 <= a_num_bytes /\
+           a_num_bytes < length a128 * 16 + 16 /\
+           4096 * a_num_bytes < pow2_32 /\
+           length p128x6 == length c128x6 /\
+           length p128 == length c128 /\
+           length p_bytes == 1 /\
+           length c_bytes == 1 /\
+           length a_bytes == 1 /\
+           is_aes_key_LE alg key /\
+
+           h = aes_encrypt_LE alg key (Mkfour 0 0 0 0) /\
+
+           // Ensured by gcm_blocks
+           8 * p_num_bytes < pow2_32 /\ 8 * a_num_bytes < pow2_32 /\
+           length_quad == reverse_bytes_quad32 (Mkfour (8 * p_num_bytes) 0 (8 * a_num_bytes) 0) /\
+          (let ctr_BE_1:quad32 = Mkfour 1 iv_BE.lo1 iv_BE.hi2 iv_BE.hi3 in
+           let ctr_BE_2:quad32 = Mkfour 2 iv_BE.lo1 iv_BE.hi2 iv_BE.hi3 in
+           let plain:seq quad32 = 
+             if p_num_bytes > (length p128x6 + length p128) * 16 then
+               append (append p128x6 p128) p_bytes
+             else
+               append p128x6 p128
+           in
+           let cipher:seq quad32 =
+             if p_num_bytes > (length p128x6 + length p128) * 16 then
+               append (append c128x6 c128) c_bytes
+             else
+               append c128x6 c128
+           in
+           let cipher_bound:nat = length p128x6 + length p128 +
+             (if p_num_bytes > (length p128x6 + length p128) * 16 then 1 else 0)
+           in
+           gctr_partial_opaque alg cipher_bound plain cipher key ctr_BE_2 /\
+
+          (let auth_raw_quads =
+             if a_num_bytes > (length a128) * 16 then append a128 a_bytes else a128
+           in
+           
+           let auth_input_bytes = slice (le_seq_quad32_to_bytes auth_raw_quads) 0 a_num_bytes in
+           let auth_padded_bytes = pad_to_128_bits auth_input_bytes in
+           let auth_quads = le_bytes_to_seq_quad32 auth_padded_bytes in
+           
+           let raw_quads = append (append auth_quads c128x6) c128 in
+           let total_bytes = (length auth_quads) * 16 + p_num_bytes in
+           let raw_quads = 
+             if p_num_bytes > (length p128x6 + length p128) * 16 then
+               let raw_quads = append raw_quads c_bytes in
+               let input_bytes = slice (le_seq_quad32_to_bytes raw_quads) 0 total_bytes in
+               let input_padded_bytes = pad_to_128_bits input_bytes in
+               le_bytes_to_seq_quad32 input_padded_bytes
+             else
+               raw_quads 
+           in
+           let final_quads = append raw_quads (create 1 length_quad) in
+           enc_hash == gctr_encrypt_block ctr_BE_1 (ghash_LE h final_quads) alg key 0               
+           )))
+  (ensures (let auth_raw_quads =
+             if a_num_bytes > (length a128) * 16 then append a128 a_bytes else a128
+           in           
+           let auth_input_bytes = slice (le_seq_quad32_to_bytes auth_raw_quads) 0 a_num_bytes in
+           let plain_raw_quads =
+             if p_num_bytes > (length p128x6 + length p128) * 16 then
+               append (append p128x6 p128) p_bytes
+             else append p128x6 p128
+           in
+           let plain_input_bytes = slice (le_seq_quad32_to_bytes plain_raw_quads) 0 p_num_bytes in
+           4096 * length auth_input_bytes < pow2_32 /\
+           4096 * length plain_input_bytes < pow2_32 /\
+           le_quad32_to_bytes enc_hash == 
+             snd (gcm_encrypt_LE alg (seq_nat32_to_seq_nat8_LE key) 
+                                 (be_quad32_to_bytes iv_BE) plain_input_bytes auth_input_bytes)))
+  =
+  let ctr_BE_1:quad32 = Mkfour 1 iv_BE.lo1 iv_BE.hi2 iv_BE.hi3 in
+  let ctr_BE_2:quad32 = Mkfour 2 iv_BE.lo1 iv_BE.hi2 iv_BE.hi3 in
+  let plain:seq quad32 = 
+    if p_num_bytes > (length p128x6 + length p128) * 16 then
+       append (append p128x6 p128) p_bytes
+    else
+      append p128x6 p128
+  in
+  let cipher:seq quad32 =
+    if p_num_bytes > (length p128x6 + length p128) * 16 then
+       append (append c128x6 c128) c_bytes
+    else
+      append c128x6 c128
+  in
+  let cipher_bound:nat = length p128x6 + length p128 +
+    (if p_num_bytes > (length p128x6 + length p128) * 16 then 1 else 0)
+  in
+  let plain_bytes = slice (le_seq_quad32_to_bytes plain) 0 p_num_bytes in
+  let cipher_bytes = slice (le_seq_quad32_to_bytes cipher) 0 p_num_bytes in
+  let auth_raw_quads =
+    if a_num_bytes > (length a128) * 16 then append a128 a_bytes else a128
+  in
+  let auth_input_bytes = slice (le_seq_quad32_to_bytes auth_raw_quads) 0 a_num_bytes in
+  let auth_padded_bytes = pad_to_128_bits auth_input_bytes in
+  let auth_quads = le_bytes_to_seq_quad32 auth_padded_bytes in
+  
+  let raw_quads = append (append auth_quads c128x6) c128 in
+  let total_bytes = (length auth_quads) * 16 + p_num_bytes in
+  let raw_quads = 
+    if p_num_bytes > (length p128x6 + length p128) * 16 then
+       let raw_quads = append raw_quads c_bytes in
+       let input_bytes = slice (le_seq_quad32_to_bytes raw_quads) 0 total_bytes in
+       let input_padded_bytes = pad_to_128_bits input_bytes in
+       le_bytes_to_seq_quad32 input_padded_bytes
+    else
+      raw_quads 
+  in
+  let final_quads = append raw_quads (create 1 length_quad) in
+  let hash = ghash_LE h final_quads in
+
+  gcm_blocks_helper_enc alg key p128x6 p128 p_bytes c128x6 c128 c_bytes auth_input_bytes p_num_bytes iv_BE;
+  //assert (cipher_bytes == fst (gcm_encrypt_LE alg (seq_nat32_to_seq_nat8_LE key) (be_quad32_to_bytes iv_BE) plain_bytes auth_input_bytes)); // Passes
+
+  if p_num_bytes > (length p128x6 + length p128) * 16 then (
+    ()
+  ) else (
+    (*
+    calc (==) {
+      append (append (append auth_quads c128x6) c128) (create 1 length_quad);
+        == { append_assoc auth_quads c128x6 c128 }
+      append (append auth_quads (append c128x6 c128)) (create 1 length_quad);
+        == { append_assoc auth_quads (append c128x6 c128) (create 1 length_quad) }
+      append auth_quads (append (append c128x6 c128) (create 1 length_quad));
+    };
+    let c = append c128x6 c128 in
+    calc (==) {
+      le_bytes_to_seq_quad32 (pad_to_128_bits (slice (le_seq_quad32_to_bytes c) 0 p_num_bytes));
+      == { assert (equal (le_seq_quad32_to_bytes c) (slice (le_seq_quad32_to_bytes c) 0 p_num_bytes)) }
+      le_bytes_to_seq_quad32 (pad_to_128_bits (le_seq_quad32_to_bytes c));
+      == { assert (pad_to_128_bits (le_seq_quad32_to_bytes c) == (le_seq_quad32_to_bytes c)) }
+      le_bytes_to_seq_quad32 (le_seq_quad32_to_bytes c);
+      == { le_bytes_to_seq_quad32_to_bytes c }
+      c;
+    };
+
+
+    calc (==) {
+      enc_hash;
+      == {}
+      gctr_encrypt_block ctr_BE_1 (ghash_LE h final_quads) alg key 0;
+      == {}
+      gctr_encrypt_block ctr_BE_1 hash alg key 0;
+      == {}
+      quad32_xor hash (aes_encrypt_LE alg key (reverse_bytes_quad32 ctr_BE_1));
+      == { reveal_opaque aes_encrypt_LE_def }
+      quad32_xor hash (aes_encrypt_le alg key (reverse_bytes_quad32 ctr_BE_1));
+      == {}
+      quad32_xor hash (aes_encrypt_BE alg key ctr_BE_1);
+    };
+
+    calc (==) {
+      gctr_encrypt_LE ctr_BE_1 (le_quad32_to_bytes hash) alg key;
+      == { gctr_encrypt_one_block ctr_BE_1 hash alg key }
+      le_seq_quad32_to_bytes (create 1 (quad32_xor hash (aes_encrypt_BE alg key ctr_BE_1)));
+      == {}
+      le_seq_quad32_to_bytes (create 1 enc_hash);
+      == { le_seq_quad32_to_bytes_of_singleton enc_hash }
+      le_quad32_to_bytes enc_hash;
+    };  
+    gcm_encrypt_LE_snd_helper iv_BE length_quad hash enc_hash plain_bytes auth_input_bytes cipher_bytes alg key;
+    *)
+    admit()
+    ()
+  );
+  admit();
+  ()
+
 
 
 let lemma_gcm_encrypt_decrypt_equiv (alg:algorithm) (key:seq nat32) (iv_BE:quad32) (plain cipher auth alleged_tag:seq nat8) : Lemma
